theories/typing/lib/panic.v
@@ -1,0 +1,25 @@
+From iris.proofmode Require Import tactics.
+From lrust.typing Require Import typing.
+Set Default Proof Using "Type".
+
+(* Minimal support for panic. Lambdarust does not support unwinding
+   the stack. Instead, we just end the current thread by not calling
+   any continuation.
+
+   Note that this is not very faithfull, because e.g., [spawn] will
+   not be notified that the thread has finished. This is why we do not
+   get into trouble with [take_mut]. *)
+
+Section panic.
+  Context `{typeG Σ}.
+
+  Definition panic : val :=
+    funrec: <> [] := #().
+
+  Lemma panic_type ty `{!TyWf ty} : typed_val panic (fn(∅) → ty).
+  Proof.
+    intros E L. iApply type_fn; [solve_typing..|]. iIntros "!# *".
+    inv_vec args.  iIntros (tid) "LFT HE Hna HL Hk HT /=". simpl_subst.
+    wp_value. done.
+  Qed.
+End panic.
